Added runST and Nik's explanation about the validity of this combinator

examples/dm4free/FStar.DM4F.Heap.ST.fst
@@ -185,6 +185,26 @@ let refine_st (#a:Type)
 (* let bad (r:ref int) = alloc #(unit -> STNull unit) (fun () -> incr r) *)
 
 
+////////////////////////////////////////////////////////////////////////////////
+//
+//  Using reification we can run an arbitrary state computation starting
+//  from an empty heap. At compilation time, this combinator ought to be
+//  treated specially and [runST e] should be compiled to [e ()]. This
+//  operation is semantically valid since the operational semantic of ST
+//  is an abstraction over the semantic of the heap after compilation.
+//
+////////////////////////////////////////////////////////////////////////////////
+abstract
+val runST :
+  (#a:Type) ->
+  (#post:(heap -> a -> heap -> Type0)) ->
+  (unit -> ST a (requires (fun h -> True)) (ensures post)) ->
+  Pure a
+    (requires True)
+    (ensures (fun x -> exists h0 h1. post h0 x h1))
+abstract
+let runST #a #post s = fst (reify (s ()) FStar.DM4F.Heap.emp)
+
 
 ////////////////////////////////////////////////////////////////////////////////
 //
